src/Concurrent/ProcessSemantics.v
@@ -13,9 +13,9 @@ Definition Mailbox : Set := list Val * list Val.
 Definition emptyBox : Mailbox := ([], []).
 Definition ProcessFlag : Set := bool.
 (* TODO: list PID -> gset PID refactoring - however, there are technical challenges *)
-Definition LiveProcess : Set := FrameStack * Redex * Mailbox * list PID * ProcessFlag.
+Definition LiveProcess : Set := FrameStack * Redex * Mailbox * gset PID * ProcessFlag.
 
-(* Instance PIDVal_eq_dec : EqDecision (PID * Val).
+Instance PIDVal_eq_dec : EqDecision (PID * Val).
 Proof.
   pose proof Val_eq_dec.
   eapply prod_eq_dec.
@@ -25,15 +25,40 @@ Defined.
 
 Hint Resolve PIDVal_eq_dec : core.
 
-Instance PIDVal_countable : Countable (PID * Val).
+Instance Val_eq_decision : EqDecision Val.
 Proof.
-  Search Countable.
+  pose proof Val_eq_dec.
+  unfold EqDecision, Decision. apply H.
 Defined.
 
-Hint Resolve PIDVal_eq_dec : core. *)
+Hint Resolve Val_eq_decision : core.
+
+
+Instance singleton_PID : Singleton PID (gset PID).
+Proof.
+  unfold Singleton.
+  intro x. exact {[x]}.
+Defined.
+
+Hint Resolve singleton_PID : core.
+
+
+(* Instance Val_countable : Countable Val.
+Proof.
+  (* TODO: technical, requires Countable Exp and mutual induction *)
+Admitted.
+
+Hint Resolve Val_countable : core.
+
+Instance PIDVal_countable : Countable (PID * Val).
+Proof.
+  apply prod_countable.
+Defined.
+
+Hint Resolve PIDVal_countable : core. *)
 
 (* TODO: rewrite this with gset too *)
-Definition DeadProcess : Set := list (PID * Val).
+Definition DeadProcess : Set := gmap PID Val.
 Definition Process : Set := LiveProcess + DeadProcess.
 
 Inductive Signal : Set :=
@@ -51,7 +76,7 @@ Inductive Action : Set :=
 (* | ADestroy (* <- this is a concurrent action *) *)
 | AArrive (sender receiver : PID) (t : Signal)
 | ASelf (ι : PID)
-| ASpawn (ι : PID) (t1 t2 : Val)
+| ASpawn (ι : PID) (t1 t2 : Val) (link : bool)
 | τ (* tau denotes confluent actions of the semantics (these are silent steps and a few other reductions) *)
 | ε (* epsilon is used for process-local silent operations (e.g., mailbox manipulation), which are NOT confluent *)
 (* | ATerminate *)
@@ -219,7 +244,7 @@ Inductive processLocalSemantics : Process -> Action -> Process -> Prop :=
   (flag = false /\ reason = normal /\ source = dest /\ reason' = reason) ->
   (*    ^------------ TODO: this check is missing from doc. *)
   inl (fs, e, mb, links, flag) -⌈ AArrive source dest (SExit reason b) ⌉->
-  inr (map (fun l => (l, reason')) links)
+  inr (gset_to_gmap reason' links)
 (* convert exit signal to message *)
 | p_exit_convert fs e mb links dest source reason b:
   (b = false /\ reason <> kill) \/
@@ -230,12 +255,12 @@ Inductive processLocalSemantics : Process -> Action -> Process -> Prop :=
 (* link received *)
 | p_link_arrived fs e mb links source dest flag:
   inl (fs, e, mb, links, flag) -⌈AArrive source dest SLink⌉->
-  inl (fs, e, mb, source :: links, flag)
+  inl (fs, e, mb, {[source]} ∪ links, flag)
 
 (* unlink received *)
 | p_unlink_arrived fs e mb links source dest flag :
   inl (fs, e, mb, links, flag) -⌈AArrive source dest SUnlink⌉->
-  inl (fs, e, mb, remove Nat.eq_dec source links, flag)
+  inl (fs, e, mb, links ∖ {[source]}, flag)
 
 (********** SIGNAL SENDING **********)
 (* message send *)
@@ -252,16 +277,17 @@ Inductive processLocalSemantics : Process -> Action -> Process -> Prop :=
 | p_link fs ι mb flag links selfι :
   inl (FParams (ICall erlang link) [] [] :: fs, RValSeq [VPid ι], mb, links, flag)
   -⌈ASend selfι ι SLink⌉->
-  inl (fs, RValSeq [ok], mb, ι :: links, flag)
+  inl (fs, RValSeq [ok], mb, {[ι]} ∪ links, flag)
 (* unlink *)
 | p_unlink fs ι mb flag links selfι :
   inl (FParams (ICall erlang unlink) [] [] :: fs, RValSeq [VPid ι], mb, links, flag) 
   -⌈ASend selfι ι SUnlink⌉->
-  inl (fs, RValSeq [ok], mb, remove Nat.eq_dec ι links, flag)
+  inl (fs, RValSeq [ok], mb, links ∖ {[ι]}, flag)
 (* DEAD PROCESSES *)
 | p_dead ι selfι links reason:
   VALCLOSED reason ->
-  inr ((ι, reason) :: links) -⌈ASend selfι ι (SExit reason true)⌉-> inr links
+  links !! ι = Some reason ->
+  inr links -⌈ASend selfι ι (SExit reason true)⌉-> inr (delete ι links)
 
 
 (********** SELF **********)
@@ -274,7 +300,13 @@ Inductive processLocalSemantics : Process -> Action -> Process -> Prop :=
 | p_spawn ι fs mb ext id vars e l flag links :
   Some vars = len l ->
   inl (FParams (ICall erlang spawn) [VClos ext id vars e] [] :: fs, RValSeq [l], mb, links, flag)
-    -⌈ASpawn ι (VClos ext id vars e) l⌉-> inl (fs, RValSeq [VPid ι], mb, links, flag)
+    -⌈ASpawn ι (VClos ext id vars e) l false⌉-> inl (fs, RValSeq [VPid ι], mb, links, flag)
+
+(* spawn_link *)
+| p_spawn_link ι fs mb ext id vars e l flag links :
+  Some vars = len l ->
+  inl (FParams (ICall erlang spawn_link) [VClos ext id vars e] [] :: fs, RValSeq [l], mb, links, flag)
+    -⌈ASpawn ι (VClos ext id vars e) l true⌉-> inl (fs, RValSeq [VPid ι], mb, {[ι]} ∪ links, flag)
 
 (********** RECEVIE **********)
 (* nonempty peeks are confluent, while empty peeks are not *)
@@ -326,7 +358,7 @@ Inductive processLocalSemantics : Process -> Action -> Process -> Prop :=
 | p_terminate v mb links flag:
   (* NOTE: "singletonness" is checked in compile time in Core Erlang *)
   inl ([], RValSeq [v], mb, links, flag) -⌈ε⌉->
-   inr (map (fun l => (l, normal)) links)
+   inr (gset_to_gmap normal links)
 
 (* exit with one parameter <- this is sequential, it's in FrameStack/Auxiliaries.v *)
 
@@ -336,7 +368,7 @@ Inductive processLocalSemantics : Process -> Action -> Process -> Prop :=
   (* NOTE: if the final result is an exception, it's reason is sent
      to the linked processes *)
   inl ([], RExc exc, mb, links, flag) -⌈ε⌉->
-   inr (map (fun l => (l, exc.1.2)) links)
+   inr (gset_to_gmap exc.1.2 links)
 
 where "p -⌈ a ⌉-> p'" := (processLocalSemantics p a p').
 
@@ -351,7 +383,7 @@ Notation "x -⌈ xs ⌉->* y" := (LabelStar processLocalSemantics x xs y) (at le
     in the equivalence. *)
 Definition spawnPIDOf (a : Action) : option PID :=
   match a with
-  | ASpawn ι _ _ => Some ι
+  | ASpawn ι _ _ _ => Some ι
   | _ => None
   end.
 
@@ -420,48 +452,134 @@ Defined.
 Definition renamePIDMb (p p' : PID) (mb : Mailbox) : Mailbox :=
   (map (renamePIDVal p p') mb.1, map (renamePIDVal p p') mb.2).
 
+Definition renamePIDPID_sym (p p' : PID) := fun s => if s =? p
+                                                     then p'
+                                                     else if s =? p'
+                                                      (* This part is needed
+                                                         for Inj eq eq *)
+                                                          then p
+                                                          else s.
+
+Instance renamePIDPID_sym_Inj p p' : Inj eq eq (renamePIDPID_sym p p').
+Proof.
+  unfold Inj. intros. unfold renamePIDPID_sym in H.
+  repeat case_match; eqb_to_eq; subst; auto; try congruence.
+Defined.
+
+Hint Resolve renamePIDPID_sym_Inj : core.
+Hint Resolve prod_map_inj : core.
+Hint Resolve id_inj : core.
+
 Definition renamePIDProc (p p' : PID) (pr : Process) : Process :=
 match pr with
 | inl (fs, r, mb, links, flag) =>
   inl (renamePIDStack p p' fs, renamePIDRed p p' r,
        renamePIDMb p p' mb,
-       map (renamePIDPID p p') links, flag)
-| inr dpr => inr (map (fun '(d, v) => (renamePIDPID p p' d, renamePIDVal p p' v)) dpr)
+       set_map (renamePIDPID p p') links, flag)
+| inr dpr => inr (kmap (renamePIDPID_sym p p') (fmap (renamePIDVal p p') dpr))
 end.
+
+Definition union_set {A C : Type} {H : Union C} {H0 : Elements C A} {H1 : Empty C} (s : A) : C := union_list (elements s).
+
+Instance gsetPID_elem_of : Elements (gset PID) (gset (gset PID)).
+Proof.
+  unfold Elements.
+  exact elements.
+Defined.
+
 
 Definition usedPIDsProc (p : Process) : gset PID :=
 match p with
 | inl (fs, r, mb, links, flag) => 
     usedPIDsStack fs ∪
     usedPIDsRed r ∪
-    list_to_set links ∪
+    links ∪
     flat_union usedPIDsVal mb.1 ∪
     flat_union usedPIDsVal mb.2
-| inr links => (* TODO: should links should be considered? - Probably *)
-    flat_union (fun x => {[x.1]} ∪ usedPIDsVal x.2) links
+| inr links => (* should links should be considered? - Definitely *)
+    (* map_fold (fun k x acc => {[k]} ∪ usedPIDsVal x ∪ acc) ∅ links <- simple, but no support with theorems *)
+    @union_set _ _ _ gsetPID_elem_of _ (map_to_set (fun k x => {[k]} ∪ usedPIDsVal x) links)
 end.
 
+Ltac renamePIDPID_case_match :=
+  unfold renamePIDPID; repeat case_match; eqb_to_eq; subst; try lia.
+Ltac renamePIDPID_case_match_hyp H :=
+  unfold renamePIDPID in H; repeat case_match; eqb_to_eq; subst; try lia.
+Ltac renamePIDPID_sym_case_match :=
+  unfold renamePIDPID_sym; repeat case_match; eqb_to_eq; subst; try lia.
+Ltac renamePIDPID_sym_case_match_hyp H :=
+  unfold renamePIDPID_sym in H; repeat case_match; eqb_to_eq; subst; try lia.
+
 Corollary isNotUsed_renamePID_proc :
-  forall p from to, from ∉ (usedPIDsProc p) -> renamePIDProc from to p = p.
+  forall p from to, from ∉ (usedPIDsProc p) ->
+    to ∉ usedPIDsProc p -> (* needed for dead processes *)
+    renamePIDProc from to p = p.
 Proof.
-  intros. destruct p; simpl.
+  intros * H Hdead. destruct p; simpl.
   * destruct l, p, p, p, m. simpl.
     simpl in H. repeat apply not_elem_of_union in H as [H ?].
     rewrite not_elem_of_flat_union in *.
     rewrite isNotUsed_renamePID_red, isNotUsed_renamePID_stack; auto.
     repeat f_equal.
     1: unfold renamePIDMb; simpl; f_equal.
-    all: rewrite <- map_id; apply map_ext_in; intros; simpl.
+    1-2: rewrite <- map_id; apply map_ext_in; intros; simpl.
     1-2: rewrite isNotUsed_renamePID_val; apply elem_of_list_In in H4; set_solver.
-    unfold renamePIDPID. break_match_goal; eqb_to_eq; subst. 2: reflexivity.
-    apply elem_of_list_In in H4. set_solver.
-  * f_equal. rewrite <- map_id; apply map_ext_in; intros; simpl. destruct a.
-    unfold usedPIDsProc in H.
-    rewrite elem_of_flat_union in H.
-    apply elem_of_list_In in H0.
-    rewrite isNotUsed_renamePID_val. 2: intro; apply H; set_solver.
-    unfold renamePIDPID. case_match; auto. eqb_to_eq; subst.
-    set_solver.
+    apply set_eq; split; intros.
+    - apply elem_of_map in H4; destruct_hyps.
+      unfold renamePIDPID in H4; renamePIDPID_case_match_hyp H4.
+      congruence. assumption.
+    - apply elem_of_map. destruct (decide (x = from)).
+      + congruence.
+      + exists x. split. by renamePIDPID_case_match. assumption.
+  * f_equal.
+    apply map_eq. intros.
+    (* TODO: Lot of boiler plate, since stdpp is not quite easily extensible with
+       helper lemmas :(  *)
+    destruct (decide (i = from)). 2: destruct (decide (i = to)).
+    - subst.
+      replace from with (renamePIDPID_sym from to to) at 1 by  renamePIDPID_sym_case_match.
+      setoid_rewrite lookup_kmap; auto.
+      setoid_rewrite lookup_fmap. simpl in *.
+      destruct (d !! to) eqn:P1. 2: destruct (d !! from) eqn:P2.
+      3: by setoid_rewrite P1; setoid_rewrite P2.
+      + exfalso. apply Hdead.
+        unfold union_set in *. apply elem_of_union_list.
+        exists ({[to]} ∪ usedPIDsVal v). split. 2: set_solver.
+        apply elem_of_elements. apply elem_of_map_to_set.
+        do 2 eexists. split. exact P1. reflexivity.
+      + exfalso. apply H.
+        unfold union_set in *. apply elem_of_union_list.
+        exists ({[from]} ∪ usedPIDsVal v). split. 2: set_solver.
+        apply elem_of_elements. apply elem_of_map_to_set.
+        do 2 eexists. split. exact P2. reflexivity.
+    - subst.
+      replace to with (renamePIDPID_sym from to from) at 1 by  renamePIDPID_sym_case_match.
+      setoid_rewrite lookup_kmap; auto.
+      setoid_rewrite lookup_fmap. simpl in *.
+      destruct (d !! to) eqn:P1. 2: destruct (d !! from) eqn:P2.
+      3: by setoid_rewrite P1; setoid_rewrite P2.
+      + exfalso. apply Hdead.
+        unfold union_set in *. apply elem_of_union_list.
+        exists ({[to]} ∪ usedPIDsVal v). split. 2: set_solver.
+        apply elem_of_elements. apply elem_of_map_to_set.
+        do 2 eexists. split. exact P1. reflexivity.
+      + exfalso. apply H.
+        unfold union_set in *. apply elem_of_union_list.
+        exists ({[from]} ∪ usedPIDsVal v). split. 2: set_solver.
+        apply elem_of_elements. apply elem_of_map_to_set.
+        do 2 eexists. split. exact P2. reflexivity.
+    - replace i with (renamePIDPID_sym from to i) at 1 by  renamePIDPID_sym_case_match.
+      setoid_rewrite lookup_kmap; auto.
+      setoid_rewrite lookup_fmap. simpl in *.
+      destruct (d !! i) eqn:P.
+      2: by setoid_rewrite P.
+      setoid_rewrite P. simpl. f_equal.
+      rewrite isNotUsed_renamePID_val; auto.
+      intro. apply H.
+      unfold union_set in *. apply elem_of_union_list.
+      exists ({[i]} ∪ usedPIDsVal v). split. 2: set_solver.
+      apply elem_of_elements. apply elem_of_map_to_set.
+      do 2 eexists. split. exact P. reflexivity.
 Qed.
 
 Corollary double_renamePID_proc :
@@ -474,19 +592,71 @@ Proof.
     rewrite double_PIDrenaming_red, double_PIDrenaming_stack; auto.
     repeat f_equal.
     1: unfold renamePIDMb; simpl; f_equal.
-    all: rewrite map_map, <- map_id; apply map_ext_in; intros; simpl.
+    1-2: rewrite map_map, <- map_id; apply map_ext_in; intros; simpl.
     1-2: rewrite double_PIDrenaming_val; apply elem_of_list_In in H4; set_solver.
-    unfold renamePIDPID. repeat case_match; eqb_to_eq; subst; try congruence.
-    apply elem_of_list_In in H4. set_solver.
-  * f_equal. rewrite map_map, <- map_id; apply map_ext_in; intros; simpl. destruct a.
-    unfold usedPIDsProc in H.
-    rewrite not_elem_of_flat_union in H.
-    apply elem_of_list_In in H0.
-    apply H in H0. simpl in H0.
-    rewrite double_PIDrenaming_val. 2: set_solver.
-    unfold renamePIDPID.
-    repeat case_match; eqb_to_eq; subst; try congruence.
-    set_solver.
+    apply set_eq; split; intros.
+    - apply elem_of_map in H4; destruct_hyps.
+      apply elem_of_map in H5; destruct_hyps.
+      unfold renamePIDPID in H4, H5; renamePIDPID_case_match_hyp H4; auto.
+      congruence.
+    - apply elem_of_map. destruct (decide (x = from)).
+      + exists to. split. by renamePIDPID_case_match.
+        apply elem_of_map. exists from. split. by renamePIDPID_case_match. by subst.
+      + exists x. split. by renamePIDPID_case_match.
+        apply elem_of_map. exists x. split. by renamePIDPID_case_match. assumption.
+  * f_equal.
+    apply map_eq. intros.
+    (* TODO: Lot of boiler plate, since stdpp is not quite easily extensible with
+       helper lemmas :(  *)
+    destruct (decide (i = from)). 2: destruct (decide (i = to)).
+    - subst.
+      replace from with (renamePIDPID_sym to from to) at 1 by  renamePIDPID_sym_case_match.
+      setoid_rewrite lookup_kmap; auto.
+      setoid_rewrite lookup_fmap. simpl in *.
+      replace to with (renamePIDPID_sym from to from) at 2 by  renamePIDPID_sym_case_match.
+      setoid_rewrite lookup_kmap; auto.
+      setoid_rewrite lookup_fmap. simpl in *.
+      destruct (d !! from) eqn:P.
+      2: by setoid_rewrite P.
+      setoid_rewrite P. simpl.
+      rewrite double_PIDrenaming_val. reflexivity.
+      intro. apply H.
+      unfold union_set in *. apply elem_of_union_list.
+      exists ({[from]} ∪ usedPIDsVal v). split. 2: set_solver.
+      apply elem_of_elements. apply elem_of_map_to_set.
+      do 2 eexists. split. exact P. reflexivity.
+    - subst.
+      replace to with (renamePIDPID_sym to from from) at 1 by  renamePIDPID_sym_case_match.
+      setoid_rewrite lookup_kmap; auto.
+      setoid_rewrite lookup_fmap. simpl in *.
+      replace from with (renamePIDPID_sym from to to) at 2 by  renamePIDPID_sym_case_match.
+      setoid_rewrite lookup_kmap; auto.
+      setoid_rewrite lookup_fmap. simpl in *.
+      destruct (d !! to) eqn:P.
+      2: by setoid_rewrite P.
+      setoid_rewrite P. simpl.
+      rewrite double_PIDrenaming_val. reflexivity.
+      intro. apply H.
+      unfold union_set in *. apply elem_of_union_list.
+      exists ({[to]} ∪ usedPIDsVal v). split. 2: set_solver.
+      apply elem_of_elements. apply elem_of_map_to_set.
+      do 2 eexists. split. exact P. reflexivity.
+    - subst.
+      replace i with (renamePIDPID_sym to from i) at 1 by  renamePIDPID_sym_case_match.
+      setoid_rewrite lookup_kmap; auto.
+      setoid_rewrite lookup_fmap. simpl in *.
+      replace i with (renamePIDPID_sym from to i) at 1 by  renamePIDPID_sym_case_match.
+      setoid_rewrite lookup_kmap; auto.
+      setoid_rewrite lookup_fmap. simpl in *.
+      destruct (d !! i) eqn:P.
+      2: by setoid_rewrite P.
+      setoid_rewrite P. simpl.
+      rewrite double_PIDrenaming_val. reflexivity.
+      intro. apply H.
+      unfold union_set in *. apply elem_of_union_list.
+      exists ({[i]} ∪ usedPIDsVal v). split. 2: set_solver.
+      apply elem_of_elements. apply elem_of_map_to_set.
+      do 2 eexists. split. exact P. reflexivity.
 Qed.
 
 Notation "e .⟦ x ↦ y ⟧ₚ" := (renamePIDProc x y e) (at level 2).
@@ -498,8 +668,8 @@ Definition renamePIDAct (from to : PID) (a : Action) : Action :=
   | AArrive sender receiver t =>
     AArrive (renamePIDPID from to sender) (renamePIDPID from to receiver) (renamePIDSignal from to t)
   | ASelf ι => ASelf (renamePIDPID from to ι)
-  | ASpawn ι t1 t2 =>
-    ASpawn (renamePIDPID from to ι) (renamePIDVal from to t1) (renamePIDVal from to t2)
+  | ASpawn ι t1 t2 lin =>
+    ASpawn (renamePIDPID from to ι) (renamePIDVal from to t1) (renamePIDVal from to t2) lin
   | x => x
   end.
 
@@ -521,7 +691,7 @@ match a with
  | ASend sender receiver t => {[sender]} ∪ {[receiver]} ∪ usedPIDsSignal t
  | AArrive sender receiver t => {[sender]} ∪ {[receiver]} ∪ usedPIDsSignal t
  | ASelf ι => {[ι]}
- | ASpawn ι t1 t2 => {[ι]} ∪ usedPIDsVal t1 ∪ usedPIDsVal t2
+ | ASpawn ι t1 t2 _ => {[ι]} ∪ usedPIDsVal t1 ∪ usedPIDsVal t2
  | _ => ∅
 end.
 
@@ -584,6 +754,28 @@ Proof.
   f_equal. now rewrite map_app.
 Qed.
 
+Lemma renamePIDPID_1 :
+  forall a b, renamePIDPID a b a = b.
+Proof.
+  unfold renamePIDPID. intros. by rewrite Nat.eqb_refl.
+Qed.
+
+Lemma renamePIDPID_sym_1 :
+  forall a b, renamePIDPID_sym a b a = b.
+Proof.
+  unfold renamePIDPID_sym. intros. by rewrite Nat.eqb_refl.
+Qed.
+
+Lemma rename_eq :
+  forall from to ι,
+  ι <> to ->
+  renamePIDPID_sym from to ι = renamePIDPID from to ι.
+Proof.
+  unfold renamePIDPID_sym, renamePIDPID. intros.
+  case_match; auto. case_match; auto.
+  eqb_to_eq; congruence.
+Qed.
+
 Opaque mailboxPush.
 (* For this theorem, freshness is needed! *)
 Theorem renamePID_is_preserved_local :
@@ -606,7 +798,7 @@ Proof.
       1-2: set_solver.
     - right. split; auto. 2: split; auto.
       + intro.
-        apply elem_of_map_iff in H2 as [x [P_1 P_2]].
+        apply elem_of_map in H2 as [x [P_1 P_2]].
         unfold renamePIDPID in P_1. repeat break_match_hyp; eqb_to_eq; subst.
         ** contradiction.
         ** repeat apply not_elem_of_union in H1 as [H1 ?]. set_solver.
@@ -614,10 +806,49 @@ Proof.
         ** contradiction.
       + unfold renamePIDPID. repeat break_match_goal; eqb_to_eq; subst; set_solver.
   * simpl.
-    replace ((map _ (map _ links))) with
-        (map (λ l : PID, (l, reason'.⟦ from ↦ to ⟧ᵥ)) (map (renamePIDPID from to) links)).
+    replace (inr _) with
+        (inr (gset_to_gmap (reason'.⟦ from ↦ to ⟧ᵥ) ((set_map (renamePIDPID from to) links) : gset PID)) : Process).
     2: {
-      now repeat rewrite map_map.
+      assert (to ∉ links) by set_solver.
+      assert (to ∉ usedPIDsVal reason) by set_solver.
+      clear -H H3.
+      f_equal. apply map_eq. intros.
+      rewrite lookup_gset_to_gmap. unfold mguard, option_guard. case_match.
+      * clear H0. apply elem_of_map in e; destruct_hyps.
+        subst. rewrite <- rename_eq by set_solver.
+        setoid_rewrite lookup_kmap; auto.
+        setoid_rewrite lookup_fmap.
+        rewrite lookup_gset_to_gmap. simpl.
+        unfold mguard, option_guard. case_match. 2: { clear H0. set_solver. }
+        reflexivity.
+      * clear H0.
+        destruct (decide (i = from)). 2: destruct (decide (i = to)).
+        - subst.
+          replace from with (renamePIDPID_sym from to to) at 1 by renamePIDPID_sym_case_match.
+          setoid_rewrite lookup_kmap; auto.
+          setoid_rewrite lookup_fmap.
+          rewrite lookup_gset_to_gmap. simpl.
+          unfold mguard, option_guard. case_match. 2: { clear H0. set_solver. }
+          by clear H0.
+        - subst.
+          replace to with (renamePIDPID_sym from to from) at 1 by renamePIDPID_sym_case_match.
+          setoid_rewrite lookup_kmap; auto.
+          setoid_rewrite lookup_fmap.
+          rewrite lookup_gset_to_gmap. simpl.
+          unfold mguard, option_guard. case_match. 2: { clear H0. set_solver. }
+          clear H0. exfalso. apply n. apply elem_of_map. exists from.
+          split. by renamePIDPID_case_match. assumption.
+        - assert (i ∉ links). {
+            intro. apply n. apply elem_of_map. exists i.
+            split. renamePIDPID_case_match. assumption.
+          }
+          replace i with (renamePIDPID_sym from to i) at 1 by
+            renamePIDPID_sym_case_match.
+          setoid_rewrite lookup_kmap; auto.
+          setoid_rewrite lookup_fmap.
+          rewrite lookup_gset_to_gmap. simpl.
+          unfold mguard, option_guard. case_match. 2: { clear H1. set_solver. }
+          by clear H1.
     }
     constructor. destruct_or!; destruct_and!; subst.
     - left. now split; auto.
@@ -626,14 +857,14 @@ Proof.
         destruct reason; simpl in *; try congruence.
         break_match_hyp; congruence.
       + intro. apply H4 in H.
-        apply elem_of_map_iff. exists source. split; auto.
+        apply elem_of_map. exists source. split; auto.
       + intro. apply H6 in H.
         clear -H. intro; destruct reason; simpl in *; try congruence.
         break_match_hyp; congruence.
     - right. right. now split; auto.
   * simpl. rewrite mailboxPush_rename. simpl.
     pose proof (p_exit_convert (renamePIDStack from to fs) (e .⟦ from ↦ to ⟧ᵣ)
-       (renamePIDMb from to mb) (map (renamePIDPID from to) links) (renamePIDPID from to dest) (renamePIDPID from to source) (reason .⟦ from ↦ to ⟧ᵥ) b).
+       (renamePIDMb from to mb) (set_map (renamePIDPID from to) links) (renamePIDPID from to dest) (renamePIDPID from to source) (reason .⟦ from ↦ to ⟧ᵥ) b).
     (* TODO: boiler plate code: *)
     destruct (from =? source) eqn:P.
     - unfold renamePIDPID in H at 6. rewrite Nat.eqb_sym in P. rewrite P in H.
@@ -642,61 +873,122 @@ Proof.
         destruct reason; simpl in *; try congruence.
         break_match_hyp; congruence.
       + right; split; auto. clear -H4.
-        apply elem_of_map_iff. exists source. split; auto.
+        apply elem_of_map. exists source. split; auto.
     - unfold renamePIDPID in H at 6. rewrite Nat.eqb_sym in P. rewrite P in H.
       apply H. destruct_or!; destruct_and!.
       + left; split; auto. clear -H4. intro.
         destruct reason; simpl in *; try congruence.
         break_match_hyp; congruence.
       + right; split; auto. clear -H4.
-        apply elem_of_map_iff. exists source. split; auto.
+        apply elem_of_map. exists source. split; auto.
   * simpl in *. repeat apply not_in_union in H1 as [H1 ?].
-    rewrite map_renamePIDPID_remove; auto. now constructor.
-    all: set_solver.
+    replace (set_map (renamePIDPID from to) ({[source]} ∪ links)) with
+      ({[renamePIDPID from to source]} ∪ set_map (renamePIDPID from to) links : gset PID) by (clear; set_solver).
+    constructor.
+  * simpl in *.
+    unfold set_map at 2. (* Why does replace not work without unfolding?? *)
+    (* TODO: extract it somehow to a separate theorem about set_map and ∖ - couldn't do it because of the tagling typeclasses *)
+    replace (list_to_set (renamePIDPID from to <$> elements (links ∖ {[source]})))
+      with ((set_map (renamePIDPID from to) links ∖ {[renamePIDPID from to source]}) : gset PID).
+    2: {
+      apply set_eq. split; intros.
+      * apply elem_of_difference in H as [H ?].
+        apply elem_of_map in H. destruct_hyps. subst.
+        destruct (decide (x0 = source)). set_solver.
+        assert (x0 ≠ to) by set_solver.
+        destruct (decide (x0 = from)).
+        - subst. renamePIDPID_case_match. renamePIDPID_case_match_hyp H2.
+          apply elem_of_map. exists from. rewrite Nat.eqb_refl. set_solver.
+        - renamePIDPID_case_match. renamePIDPID_case_match_hyp H2.
+          apply elem_of_map. exists x0. case_match; eqb_to_eq; set_solver.
+          apply elem_of_map. exists x0. case_match; eqb_to_eq; set_solver.
+      * apply elem_of_map in H. destruct_hyps. subst.
+        assert (x0 ≠ to) by set_solver.
+        destruct (decide (x0 = from)).
+        - subst. renamePIDPID_case_match. set_solver.
+          apply elem_of_difference. split. 2: set_solver.
+          apply elem_of_map. exists from. rewrite Nat.eqb_refl. split. reflexivity.
+          set_solver.
+        - subst. renamePIDPID_case_match.
+          + apply elem_of_difference. split. 2: set_solver.
+            apply elem_of_map. exists x0. case_match; eqb_to_eq; set_solver.
+          + apply elem_of_difference. split. 2: set_solver.
+            apply elem_of_map. exists x0. case_match; eqb_to_eq; set_solver.
+    }
+    constructor.
   * simpl in *. destruct Nat.eqb eqn:P; eqb_to_eq; subst.
-    - replace (renamePIDPID ι to ι) with to by (unfold renamePIDPID; now rewrite Nat.eqb_refl). apply p_send. now apply renamePID_preserves_scope.
-    - replace (renamePIDPID from to ι) with ι. 2: {
-        unfold renamePIDPID. apply Nat.eqb_neq in P. rewrite Nat.eqb_sym in P.
-        now rewrite P.
-      }
-      apply p_send. now apply renamePID_preserves_scope.
-  * simpl in *. destruct Nat.eqb eqn:P; eqb_to_eq; subst.
-    - replace (renamePIDPID ι to ι) with to by (unfold renamePIDPID; now rewrite Nat.eqb_refl). constructor. now apply renamePID_preserves_scope.
-    - replace (renamePIDPID from to ι) with ι. 2: {
-        unfold renamePIDPID. apply Nat.eqb_neq in P. rewrite Nat.eqb_sym in P.
-        now rewrite P.
-      }
+    - replace (renamePIDPID ι to ι) with to by (renamePIDPID_case_match). constructor. now apply renamePID_preserves_scope.
+    - replace (renamePIDPID from to ι) with ι by renamePIDPID_case_match.
       constructor. now apply renamePID_preserves_scope.
   * simpl in *. destruct Nat.eqb eqn:P; eqb_to_eq; subst.
-    - replace (renamePIDPID ι to ι) with to by (unfold renamePIDPID; now rewrite Nat.eqb_refl). constructor.
-    - replace (renamePIDPID from to ι) with ι. 2: {
-        unfold renamePIDPID. apply Nat.eqb_neq in P. rewrite Nat.eqb_sym in P.
-        now rewrite P.
-      }
+    - replace (renamePIDPID ι to ι) with to by (renamePIDPID_case_match).
+      constructor. by apply renamePID_preserves_scope.
+    - replace (renamePIDPID from to ι) with ι by renamePIDPID_case_match.
+      constructor. by apply renamePID_preserves_scope.
+  * simpl in *. rewrite set_map_union_L. simpl.
+    destruct Nat.eqb eqn:P; eqb_to_eq; subst.
+    - rewrite set_map_singleton_L.
+      replace (renamePIDPID ι to ι) with to by renamePIDPID_case_match.
       constructor.
-  * simpl in *. rewrite map_renamePIDPID_remove; auto.
-    2: set_solver.
-    destruct Nat.eqb eqn:P; eqb_to_eq; subst. 3: set_solver.
-    - replace (renamePIDPID ι to ι) with to by (unfold renamePIDPID; now rewrite Nat.eqb_refl). constructor.
-    - replace (renamePIDPID from to ι) with ι. 2: {
-        unfold renamePIDPID. apply Nat.eqb_neq in P. rewrite Nat.eqb_sym in P.
-        now rewrite P.
-      }
+    - rewrite set_map_singleton_L.
+      replace (renamePIDPID from to ι) with ι by renamePIDPID_case_match.
       constructor.
-  * simpl in *. constructor. now apply renamePID_preserves_scope.
+  * simpl in *.
+    unfold set_map at 2. (* Why does replace not work without unfolding?? *)
+    (* TODO: extract it somehow to a separate theorem about set_map and ∖ - couldn't do it because of the tagling typeclasses *)
+    replace (list_to_set (renamePIDPID from to <$> elements (links ∖ {[ι]})))
+      with ((set_map (renamePIDPID from to) links ∖ {[renamePIDPID from to ι]}) : gset PID).
+    2: {
+      apply set_eq. split; intros.
+      * apply elem_of_difference in H as [H ?].
+        apply elem_of_map in H. destruct_hyps. subst.
+        destruct (decide (x0 = ι)). set_solver.
+        assert (x0 ≠ to) by set_solver.
+        destruct (decide (x0 = from)).
+        - subst. renamePIDPID_case_match. renamePIDPID_case_match_hyp H2.
+          apply elem_of_map. exists from. rewrite Nat.eqb_refl. set_solver.
+        - renamePIDPID_case_match. renamePIDPID_case_match_hyp H2.
+          apply elem_of_map. exists x0. case_match; eqb_to_eq; set_solver.
+          apply elem_of_map. exists x0. case_match; eqb_to_eq; set_solver.
+      * apply elem_of_map in H. destruct_hyps. subst.
+        assert (x0 ≠ to) by set_solver.
+        destruct (decide (x0 = from)).
+        - subst. renamePIDPID_case_match. set_solver.
+          apply elem_of_difference. split. 2: set_solver.
+          apply elem_of_map. exists from. rewrite Nat.eqb_refl. split. reflexivity.
+          set_solver.
+        - subst. renamePIDPID_case_match.
+          + apply elem_of_difference. split. 2: set_solver.
+            apply elem_of_map. exists x0. case_match; eqb_to_eq; set_solver.
+          + apply elem_of_difference. split. 2: set_solver.
+            apply elem_of_map. exists x0. case_match; eqb_to_eq; set_solver.
+    }
+    destruct Nat.eqb eqn:P; eqb_to_eq; subst.
+    - replace (renamePIDPID ι to ι) with to by renamePIDPID_case_match.
+      constructor.
+    - replace (renamePIDPID from to ι) with ι by renamePIDPID_case_match.
+    constructor.
+  * simpl in *.
+    setoid_rewrite fmap_delete.
+    setoid_rewrite kmap_delete; auto.
+    rewrite rename_eq. 2: set_solver. apply p_dead.
+    - by apply renamePID_preserves_scope.
+    - setoid_rewrite lookup_kmap_Some; auto.
+      exists ι. split. rewrite rename_eq. 2: set_solver. reflexivity.
+      setoid_rewrite lookup_fmap. by setoid_rewrite H3.
   * simpl in *. destruct Nat.eqb eqn:P; eqb_to_eq; subst.
     - replace (renamePIDPID ι to ι) with to by (unfold renamePIDPID; now rewrite Nat.eqb_refl). constructor.
-    - replace (renamePIDPID from to ι) with ι. 2: {
-        unfold renamePIDPID. apply Nat.eqb_neq in P. rewrite Nat.eqb_sym in P.
-        now rewrite P.
-      }
+    - replace (renamePIDPID from to ι) with ι by renamePIDPID_case_match.
       constructor.
   * simpl in *. destruct Nat.eqb eqn:P; eqb_to_eq; subst.
-    - replace (renamePIDPID ι to ι) with to by (unfold renamePIDPID; now rewrite Nat.eqb_refl). constructor. now rewrite len_renamePID.
-    - replace (renamePIDPID from to ι) with ι. 2: {
-        unfold renamePIDPID. apply Nat.eqb_neq in P. rewrite Nat.eqb_sym in P.
-        now rewrite P.
-      }
+    - replace (renamePIDPID ι to ι) with to by  renamePIDPID_case_match. constructor. now rewrite len_renamePID.
+    - replace (renamePIDPID from to ι) with ι by renamePIDPID_case_match.
+      constructor. now rewrite len_renamePID.
+  * simpl in *.
+    rewrite set_map_union_L, set_map_singleton_L.
+    destruct Nat.eqb eqn:P; eqb_to_eq; subst.
+    - replace (renamePIDPID ι to ι) with to by  renamePIDPID_case_match. constructor. now rewrite len_renamePID.
+    - replace (renamePIDPID from to ι) with ι by renamePIDPID_case_match.
       constructor. now rewrite len_renamePID.
   * simpl. apply p_recv_peek_message_ok. rewrite peekMessage_renamePID, H2. reflexivity.
   * simpl. constructor. rewrite peekMessage_renamePID, H2. reflexivity.
@@ -708,22 +1000,49 @@ Proof.
   * simpl. destruct flag; simpl; apply p_set_flag.
     all: destruct v; inv H2; simpl; auto.
   * simpl.
-    replace (map _ (map _ _)) with
-      (map (λ l, (l, VLit "normal"%string)) (map (renamePIDPID from to) links)).
-    apply p_terminate.
-    repeat rewrite map_map. now simpl.
-  * simpl. destruct exc, p.
-    replace (map _ (map _ _)) with
-      (map (λ l, (l, (e, v0 .⟦ from ↦ to ⟧ᵥ, v .⟦ from ↦ to ⟧ᵥ).1.2)) (map (renamePIDPID from to) links)).
-    apply p_terminate_exc.
-    repeat rewrite map_map. now simpl.
+    rewrite fmap_gset_to_gmap.
+    replace (inr _) with
+      (inr (gset_to_gmap normal (set_map (renamePIDPID from to) links)) : Process).
+    2: {
+      f_equal. apply map_eq. intros.
+      rewrite lookup_gset_to_gmap. unfold mguard, option_guard. case_match.
+      * clear H.
+        apply elem_of_map in e. destruct_hyps. subst.
+        rewrite <- rename_eq. 2: set_solver.
+        setoid_rewrite lookup_kmap; auto.
+        rewrite lookup_gset_to_gmap. unfold mguard, option_guard. case_match.
+        all: clear H; set_solver.
+      * clear H. symmetry. apply lookup_kmap_None; auto.
+        intros. subst.
+        apply lookup_gset_to_gmap_None.
+        intro. apply n. apply elem_of_map. eexists. split.
+        rewrite rename_eq. 2: set_solver.
+        reflexivity. assumption.
+    }
+    constructor.
+  * simpl. destruct exc, p. simpl.
+    rewrite fmap_gset_to_gmap.
+    replace (inr _) with
+      (inr (gset_to_gmap v0 .⟦ from ↦ to ⟧ᵥ (set_map (renamePIDPID from to) links)) : Process).
+    2: {
+      f_equal. apply map_eq. intros.
+      rewrite lookup_gset_to_gmap. unfold mguard, option_guard. case_match.
+      * clear H.
+        apply elem_of_map in e0. destruct_hyps. subst.
+        rewrite <- rename_eq. 2: set_solver.
+        setoid_rewrite lookup_kmap; auto.
+        rewrite lookup_gset_to_gmap. unfold mguard, option_guard. case_match.
+        all: clear H; set_solver.
+      * clear H. symmetry. apply lookup_kmap_None; auto.
+        intros. subst.
+        apply lookup_gset_to_gmap_None.
+        intro. apply n. apply elem_of_map. eexists. split.
+        rewrite rename_eq. 2: set_solver.
+        reflexivity. assumption.
+    }
+    constructor.
 Qed.
 Transparent mailboxPush.
-
-Ltac renamePIDPID_case_match :=
-  unfold renamePIDPID; repeat case_match; eqb_to_eq; subst; try lia.
-Ltac renamePIDPID_case_match_hyp H :=
-  unfold renamePIDPID in H; repeat case_match; eqb_to_eq; subst; try lia.
 
 Corollary renamePID_id_proc :
   forall pr p, renamePIDProc p p pr = pr.
@@ -733,14 +1052,25 @@ Proof.
     rewrite renamePID_id_stack, renamePID_id_red. f_equal.
     f_equal. f_equal. f_equal.
     - destruct m; unfold renamePIDMb. simpl. f_equal.
+      + rewrite <- (map_id l) at 2. apply map_ext_in_iff. intros.
+        by rewrite renamePID_id_val.
       + rewrite <- (map_id l0) at 2. apply map_ext_in_iff. intros.
         by rewrite renamePID_id_val.
-      + rewrite <- (map_id l1) at 2. apply map_ext_in_iff. intros.
-        by rewrite renamePID_id_val.
-    - rewrite <- (map_id l) at 2. apply map_ext_in_iff. intros.
-      renamePIDPID_case_match.
-  * f_equal. rewrite <- (map_id d) at 2. apply map_ext_in_iff. intros.
-    destruct a. rewrite renamePID_id_val. by renamePIDPID_case_match.
+    - (* TODO: set_map_id *)
+      apply set_eq. split; intros.
+      + apply elem_of_map in H. destruct_hyps. renamePIDPID_case_match_hyp H;
+        auto.
+      + apply elem_of_map. exists x. split; auto.
+        renamePIDPID_case_match.
+  * f_equal.
+    apply map_eq. intros.
+    destruct (d !! i) eqn:P; setoid_rewrite P.
+    - apply lookup_kmap_Some; auto. exists i. split.
+      + renamePIDPID_sym_case_match.
+      + setoid_rewrite lookup_fmap. setoid_rewrite P.
+        simpl. by rewrite renamePID_id_val.
+    - apply lookup_kmap_None; auto. intros.
+      setoid_rewrite lookup_fmap. renamePIDPID_sym_case_match_hyp H; by setoid_rewrite P.
 Qed.
 
 Corollary renamePID_id_sig :
@@ -818,7 +1148,7 @@ Proof.
 Qed.
 
 Corollary renamePID_swap_proc :
-  forall p from1 from2 to1 to2, from1 ≠ from2 -> from1 ≠ to2 -> from2 ≠ to1 ->
+  forall p from1 from2 to1 to2, from1 ≠ from2 -> from1 ≠ to2 -> from2 ≠ to1 -> to1 ≠ to2 ->
                renamePIDProc from1 to1 (renamePIDProc from2 to2 p) =
                renamePIDProc from2 to2 (renamePIDProc from1 to1 p).
 Proof.
@@ -831,12 +1161,100 @@ Proof.
       repeat rewrite map_map. f_equal.
       + apply map_ext_in_iff. intros. by rewrite renamePID_swap_val.
       + apply map_ext_in_iff. intros. by rewrite renamePID_swap_val.
-    - repeat rewrite map_map. apply map_ext_in_iff. intros.
-      renamePIDPID_case_match.
+    - apply set_eq. split; intros X; apply elem_of_map in X; destruct_hyps; subst;
+        apply elem_of_map in H4; destruct_hyps; subst.
+      + destruct (decide (x = from1)). 2: destruct (decide (x = from2)).
+        ** apply elem_of_map. exists to1. split.
+           renamePIDPID_case_match. apply elem_of_map.
+           exists from1. split.
+           renamePIDPID_case_match. by subst.
+        ** apply elem_of_map. exists from2. split.
+           renamePIDPID_case_match. apply elem_of_map.
+           exists from2. split.
+           renamePIDPID_case_match. by subst.
+        ** apply elem_of_map. exists x. split.
+           renamePIDPID_case_match. apply elem_of_map.
+           exists x. split.
+           renamePIDPID_case_match. by subst.
+      + destruct (decide (x = from1)). 2: destruct (decide (x = from2)).
+        ** apply elem_of_map. exists from1. split.
+           renamePIDPID_case_match. apply elem_of_map.
+           exists from1. split.
+           renamePIDPID_case_match. by subst.
+        ** apply elem_of_map. exists to2. split.
+           renamePIDPID_case_match. apply elem_of_map.
+           exists from2. split.
+           renamePIDPID_case_match. by subst.
+        ** apply elem_of_map. exists x. split.
+           renamePIDPID_case_match. apply elem_of_map.
+           exists x. split.
+           renamePIDPID_case_match. by subst.
   * intros. simpl. f_equal.
-    repeat rewrite map_map. apply map_ext_in_iff. intros. destruct a. f_equal.
-    renamePIDPID_case_match.
-    by rewrite renamePID_swap_val.
+    apply map_eq. intros.
+    (* Solution strategy is analogous for these 5 cases *)
+    destruct (decide (i = from1)). 2: destruct (decide (i = from2)).
+    3: destruct (decide (i = to1)). 4: destruct (decide (i = to2)).
+    all: subst.
+    - replace from1 with (renamePIDPID_sym from1 to1 to1) at 1 by renamePIDPID_sym_case_match.
+      setoid_rewrite lookup_kmap; auto.
+      replace from1 with (renamePIDPID_sym from2 to2 from1) at 2 by renamePIDPID_sym_case_match.
+      setoid_rewrite lookup_kmap; auto.
+      setoid_rewrite lookup_fmap.
+      replace to1 with (renamePIDPID_sym from2 to2 to1) at 2 by renamePIDPID_sym_case_match.
+      setoid_rewrite lookup_kmap; auto.
+      replace from1 with (renamePIDPID_sym from1 to1 to1) at 2 by renamePIDPID_sym_case_match.
+      setoid_rewrite lookup_kmap; auto.
+      setoid_rewrite lookup_fmap. destruct (d !! to1) eqn:P; setoid_rewrite P; simpl.
+      2: reflexivity.
+      1: by rewrite renamePID_swap_val.
+    - replace from2 with (renamePIDPID_sym from1 to1 from2) at 1 by renamePIDPID_sym_case_match.
+      setoid_rewrite lookup_kmap; auto.
+      replace from2 with (renamePIDPID_sym from2 to2 to2) at 4 by renamePIDPID_sym_case_match.
+      setoid_rewrite lookup_kmap; auto.
+      setoid_rewrite lookup_fmap.
+      replace from2 with (renamePIDPID_sym from2 to2 to2) at 1 by renamePIDPID_sym_case_match.
+      setoid_rewrite lookup_kmap; auto.
+      replace to2 with (renamePIDPID_sym from1 to1 to2) at 4 by renamePIDPID_sym_case_match.
+      setoid_rewrite lookup_kmap; auto.
+      setoid_rewrite lookup_fmap. destruct (d !! to2) eqn:P; setoid_rewrite P; simpl.
+      2: reflexivity.
+      1: by rewrite renamePID_swap_val.
+    - replace to1 with (renamePIDPID_sym from1 to1 from1) at 1 by renamePIDPID_sym_case_match.
+      setoid_rewrite lookup_kmap; auto.
+      replace to1 with (renamePIDPID_sym from2 to2 to1) at 2 by renamePIDPID_sym_case_match.
+      setoid_rewrite lookup_kmap; auto.
+      setoid_rewrite lookup_fmap.
+      replace from1 with (renamePIDPID_sym from2 to2 from1) at 2 by renamePIDPID_sym_case_match.
+      setoid_rewrite lookup_kmap; auto.
+      replace to1 with (renamePIDPID_sym from1 to1 from1) at 2 by renamePIDPID_sym_case_match.
+      setoid_rewrite lookup_kmap; auto.
+      setoid_rewrite lookup_fmap. destruct (d !! from1) eqn:P; setoid_rewrite P; simpl.
+      2: reflexivity.
+      1: by rewrite renamePID_swap_val.
+    - replace to2 with (renamePIDPID_sym from1 to1 to2) at 1 by renamePIDPID_sym_case_match.
+      setoid_rewrite lookup_kmap; auto.
+      replace to2 with (renamePIDPID_sym from2 to2 from2) at 4 by renamePIDPID_sym_case_match.
+      setoid_rewrite lookup_kmap; auto.
+      setoid_rewrite lookup_fmap.
+      replace to2 with (renamePIDPID_sym from2 to2 from2) at 1 by renamePIDPID_sym_case_match.
+      setoid_rewrite lookup_kmap; auto.
+      replace from2 with (renamePIDPID_sym from1 to1 from2) at 4 by renamePIDPID_sym_case_match.
+      setoid_rewrite lookup_kmap; auto.
+      setoid_rewrite lookup_fmap. destruct (d !! from2) eqn:P; setoid_rewrite P; simpl.
+      2: reflexivity.
+      1: by rewrite renamePID_swap_val.
+    - replace i with (renamePIDPID_sym from1 to1 i) at 1 by renamePIDPID_sym_case_match.
+      setoid_rewrite lookup_kmap; auto.
+      replace i with (renamePIDPID_sym from2 to2 i) at 2 by renamePIDPID_sym_case_match.
+      setoid_rewrite lookup_kmap; auto.
+      setoid_rewrite lookup_fmap.
+      replace i with (renamePIDPID_sym from2 to2 i) at 1 by renamePIDPID_sym_case_match.
+      setoid_rewrite lookup_kmap; auto.
+      replace i with (renamePIDPID_sym from1 to1 i) at 2 by renamePIDPID_sym_case_match.
+      setoid_rewrite lookup_kmap; auto.
+      setoid_rewrite lookup_fmap. destruct (d !! i) eqn:P; setoid_rewrite P; simpl.
+      2: reflexivity.
+      1: by rewrite renamePID_swap_val.
 Qed.
 
 Corollary usedPIDsSig_rename :
@@ -878,22 +1296,31 @@ Proof.
   * destruct l, p0, p0, p0; simpl.
     rewrite usedPIDsStack_rename, usedPIDsRed_rename. destruct m. simpl.
     do 2 rewrite usedPIDsVal_flat_union.
-    remember (flat_union _ l0) as X. remember (flat_union _ l1) as Y.
+    remember (flat_union _ l) as X. remember (flat_union _ l0) as Y.
     clear HeqX HeqY.
-    replace (list_to_set (map (renamePIDPID p p') l)) with
-                                         ((if (decide (p ∈ l))
-                                          then {[p']} ∪ list_to_set l ∖ {[p]}
-                                          else list_to_set l ∖ {[p]}) : gset PID).
+    replace (set_map (renamePIDPID p p') g) with
+                                         ((if (decide (p ∈ g))
+                                          then {[p']} ∪ g ∖ {[p]}
+                                          else g ∖ {[p]}) : gset PID).
     2: {
-      induction l; destruct decide.
-      * set_solver.
-      * set_solver.
-      * destruct decide. 2: set_solver.
-        simpl. unfold renamePIDPID. case_match; eqb_to_eq; subst; set_solver.
-      * destruct decide.
-        - assert (p = a) by set_solver. subst.
-          simpl. unfold renamePIDPID. rewrite Nat.eqb_refl. set_solver.
-        - simpl. unfold renamePIDPID. case_match; eqb_to_eq; subst; set_solver.
+      case_match; clear H; apply set_eq; split; intros.
+      * apply elem_of_union in H as [|].
+        - assert (x = p') by set_solver. subst.
+          apply elem_of_map. exists p. split; by renamePIDPID_case_match.
+        - apply elem_of_difference in H as [? ?].
+          apply elem_of_map. exists x. split. renamePIDPID_case_match. set_solver.
+          assumption.
+      * apply elem_of_map in H. destruct_hyps. subst.
+        renamePIDPID_case_match.
+        - set_solver.
+        - set_solver.
+      * apply elem_of_difference in H as [? ?].
+        apply elem_of_map. exists x. split. renamePIDPID_case_match. set_solver.
+        assumption.
+      * apply elem_of_map in H. destruct_hyps. subst.
+        renamePIDPID_case_match.
+        - set_solver.
+        - set_solver.
     }
     repeat destruct decide; set_solver. (* NOTE: this line takes long time to compile *)
   * admit.
